theories/Set.ec
@@ -1,388 +1,323 @@
 require import Int.
 require import Fun.
 
-type 'a t.
+(* For this specification, almost everything is axiomatized.
+   This is a prime candidate for 1) realization, and 2) refinement types. *)
 
-cnst empty : 'a t.
+type 'a set.
 
-op add    : ('a, 'a t) -> 'a t.
+(* These will all be axiomatized *)
+cnst empty: 'a set.
+op add: ('a, 'a set) -> 'a set.
+op pick: 'a set -> 'a.
+op rm: ('a, 'a set) -> 'a set.
+op union: ('a set,'a set) -> 'a set.
+op inter: ('a set, 'a set) -> 'a set.
+op mem: ('a, 'a set) -> bool.
+op card: 'a set -> int.
 
-op singleton (x:'a) : 'a t = add x empty.
+(* Derived operators and predicates *)
+op singleton(x:'a): 'a set = add x empty.
+op is_empty(X:'a set): bool = X = empty.
+pred cPmem(X, x:'a) = mem x X.
 
-op pick   : 'a t -> 'a.
-op rm     : ('a, 'a t) -> 'a t.
-op union  : ('a t, 'a t) -> 'a t.
-op inter  : ('a t, 'a t) -> 'a t.
+(* "Induction Principle" *)
+axiom Set_ind: forall (P:('a set) cPred),
+  P empty =>
+  (forall x S, !mem x S => P S => P (add x S)) =>
+  forall S, P S.
 
-op is_empty : 'a t -> bool.
-axiom is_empty_empty : forall (X : 'a t), is_empty X <=> X = empty.
+(* Extentional Equality *)
+pred [==] (X1 X2:'a set) = forall (x:'a),
+  mem x X1 <=> mem x X2.
 
+lemma eq_refl: forall (X:'a set), X == X.
 
-op mem      : ('a, 'a t) -> bool.
-op Pmem (X:'a t, x:'a) : bool = mem x X.
+lemma eq_sym: forall (X Y:'a set), X == Y => Y == X.
 
-axiom Set_ind : forall (P : ('a t) cPred),
-P empty =>
-(forall (S : 'a t, x : 'a), !mem x S => P S => P (add x S)) =>
- forall (S : 'a t), P S.
+lemma eq_trans: forall (X Y Z:'a set),
+  X == Y => Y == Z => X == Z.
 
-op card     : 'a t -> int.
-axiom card1 : card<:'a> empty = 0.
-axiom cadr2 : forall (S : 'a t, x : 'a), mem x S => card(S) = 1 + card(rm x S).
+axiom extentionality: forall (X1 X2:'a set),
+  X1 == X2 => X1 = X2.
 
-pred [==] (X1:'a t, X2:'a t) = 
- forall (x:'a), mem x X1 <=> mem x X2.
+(* Subset *)
+pred [<=] (X1 X2:'a set) = forall x,
+  mem x X1 => mem x X2.
 
-pred ext_eq (X1:'a t, X2:'a t) = X1 == X2. 
+lemma sub_refl: forall (X:'a set), X <= X.
 
- (* extentional equality is an equivalence relation*)
-lemma eq_refl :
- forall (X:'a t), X == X.
+lemma sub_anti_sym: forall (X Y:'a set),
+  X <= Y => Y <= X => X == Y.
 
-lemma eq_sym :
- forall (X Y:'a t), X == Y => Y == X.
+lemma sub_trans: forall (X Y Z:'a set),
+  X <= Y => Y <= Z => X <= Z.
 
+(** Specification of operators *)
+(* empty *)
+axiom empty_mem: forall (x:'a), !mem x empty.
 
-lemma eq_trans :
- forall (X Y Z:'a t), X == Y => Y == Z => X == Z.
+lemma empty_subset: forall (X:'a set), empty <= X.
 
+(* add *)
+axiom add_mem: forall (x y:'a) X, 
+  mem x (add y X) <=> mem x X \/ x = y.
 
-pred [<=] (X1:'a t, X2:'a t) = 
- forall (x:'a), mem x X1 => mem x X2.
+axiom add_card: forall (x:'a) X, 
+  !mem x X => card (add x X) = card X + 1.
 
- (* subset defines a Poset *)
-lemma sub_refl :
- forall (X:'a t), X <= X.
-
-lemma sub_anti_sym : 
- forall (X Y:'a t), X <= Y => Y <= X => X == Y.
-
-lemma sub_trans :
- forall (X Y Z:'a t), X <= Y => Y <= Z => X <= Z.
-
-axiom extentionality : 
- forall (X1:'a t, X2:'a t),
-X1 = X2 <=> X1 == X2.
-
-
- (* Specification of is_empty *)
-axiom is_empty_mem : forall (X:'a t), 
- is_empty X <=> forall (x:'a), !mem x X.
-
- (* local *) pred P_is_empty_card (X : 'a t) =
-card X = 0 => is_empty X.
-
- (* Specification of empty *)
-
-lemma empty_subset : forall(X:'a t),
- empty <= X.
-
- (* FIXME lemma *)
-lemma empty_mem  : forall (x:'a), !mem x empty.
-
-axiom empty_card : card<:'a>(empty) = 0.
-
- (* Specification of add *)
-
-axiom add_mem : forall (x:'a, y:'a, X:'a t), 
- mem x (add y X) <=> mem x X || x = y.
-
-
-axiom add_card : forall (x:'a, X:'a t), 
- !mem x X => card (add x X) = card X + 1.
-
-lemma mem_add_aux : forall (x:'a, X:'a t),
-mem x X => X == add x X.
-
-lemma mem_add : forall (x:'a, X:'a t),
-mem x X => X = add x X.
-
-lemma add_subset : forall  (x:'a, X:'a t),
- X <= add x X.
-
-lemma singleton_card : forall (x:'a),
-card (singleton x) = 1.
-
- (* local *) pred P_card_pos (X : 'a t) = 0 <= card X.
-lemma card_pos : forall (X:'a t), 0 <= card X
+lemma mem_add: forall (x:'a) X,
+  mem x X => X = add x X
 proof.
- intros X.
- cut H : (P_card_pos X).
- apply Set_ind<:'a>(P_card_pos,_,_,X);trivial.
- trivial.
+intros x X x_in_X;
+  apply extentionality<:'a> (X,(add x X),_);
+  trivial.
 save.
 
+lemma add_subset: forall (x:'a) X,
+  X <= add x X.
 
-  (* filter *)
-op filter : ('a cPred, 'a t) -> 'a t.
+(* card *)
+axiom card_empty: card<:'a> empty = 0.
+axiom card_rm: forall (x:'a) S, mem x S => card S = 1 + card(rm x S).
 
-axiom filter_mem : forall (P:'a cPred, X:'a t, x:'a),
- mem x (filter P X) <=> (mem x X && P x).
+pred (* local *) cP_card_pos (X:'a set) = 0 <= card X.
+lemma card_pos: forall (X:'a set), 0 <= card X
+proof.
+intros X;cut IH: (cP_card_pos X);
+[ apply Set_ind<:'a>(cP_card_pos,_,_,X);trivial |
+  trivial ].
+save.
 
-axiom filter_card : forall (P:'a cPred, X : 'a t), 
-card (filter P X) = card X - card(filter (cPnot P) X). 
+(* singleton *)
+lemma singleton_card: forall (x:'a),
+  card (singleton x) = 1.
 
-axiom filter_Peq_in : forall (x:'a, X:'a t),
-mem x X =>
-filter (cPeq x) X = singleton x.
+(* filter *)
+op filter: ('a cPred,'a set) -> 'a set.
 
-axiom filter_Peq_card_in : forall (x:'a, X:'a t),
-mem x X =>
-card (filter (cPeq x) X) = 1.
+axiom filter_mem: forall (x:'a) P X,
+  mem x (filter P X) <=> (mem x X /\ P x).
 
-lemma filter_subset : forall (P:'a cPred, X:'a t),
+axiom filter_card: forall (P:'a cPred) X, 
+  card (filter P X) = card X - card (filter (cPnot P) X). 
+
+axiom filter_cPeq_in: forall (x:'a) X,
+  mem x X => filter (cPeq x) X = singleton x.
+
+axiom filter_cPeq_card_in : forall (x:'a) X,
+  mem x X => card (filter (cPeq x) X) = 1.
+
+lemma filter_subset: forall (P:'a cPred) X,
  filter P X <= X.
 
- (* facts about pick *)
-axiom pick_spec : forall (X : 'a t), 
- X <> empty => mem (pick X) X.
+(* pick *)
+axiom pick_spec: forall (X:'a set), 
+  X <> empty => mem (pick X) X.
 
-lemma pick_singleton : forall (x : 'a), 
-pick (singleton x) = x.
+lemma pick_singleton: forall (x:'a), 
+  pick (singleton x) = x.
 
- (* facts about rm *)
-axiom rm_spec_not_mem : forall(X :'a t, x: 'a),
- !mem x X => rm x X = X.
+(* rm *)
+axiom rm_spec_not_mem: forall (x:'a) X,
+  !mem x X => rm x X = X.
 
-axiom rm_spec_mem : forall(X :'a t, x: 'a),
-mem x X => add x (rm x X) = X.
+axiom rm_spec_mem: forall (x:'a) X,
+  mem x X => add x (rm x X) = X.
 
-axiom rm_mem : forall (X : 'a t, x : 'a),
- !mem x (rm x X).
+axiom rm_mem: forall (x:'a) X,
+  !mem x (rm x X).
 
-lemma rm_subs :  forall (X : 'a t, x : 'a),
- rm x X <= X.
+lemma rm_subs: forall (x:'a) X,
+  rm x X <= X.
 
-lemma rm_card :  forall (X : 'a t, x : 'a),
- card(rm x X) <= card X.
+lemma rm_card: forall (x:'a) X,
+  card(rm x X) <= card X.
 
-lemma card_non_empty : forall (X : 'a t),
- forall (x :'a),
-mem x X => card<:'a> X = 1 + card (rm x X).
+lemma card_non_empty: forall (x:'a) X,
+  mem x X => card X = 1 + card (rm x X).
 
-lemma is_empty_card : forall (X:'a t),
-card X = 0 => is_empty X 
+pred (* local *) cP_is_empty_card(X:'a set) = card X = 0 => is_empty X.
+lemma is_empty_card: forall (X:'a set),
+  card X = 0 => is_empty X 
 proof.
- intros X.
- cut H : (P_is_empty_card X).
- apply Set_ind<:'a>(P_is_empty_card,_,_,X);trivial.
- trivial.
+intros X;cut IH: (cP_is_empty_card X);
+[ apply Set_ind<:'a>(cP_is_empty_card,_,_,X);trivial |
+  trivial ].
 save.
 
-  (* union *) 
-axiom union_mem : forall(X:'a t, Y:'a t, x: 'a),
- mem x (union X Y) <=> (mem x X || mem x Y).
+(* union *) 
+axiom union_mem: forall (x:'a) X Y,
+  mem x (union X Y) <=> (mem x X \/ mem x Y).
 
-lemma union_empty : forall(X :'a t),
-union X empty = X
+lemma union_empty: forall (X:'a set),
+  union X empty = X
 proof.
- intros X.
- cut H : (union X empty == X).
- trivial.
- trivial.
+intros X;
+  apply extentionality<:'a> ((union X empty),X,_);
+  trivial.
 save.
 
-lemma union_empty_aux : forall(X :'a t),
-union X empty == X.
-
-
-lemma union_comm1 : forall(X:'a t, Y:'a t),
-union X Y == union Y X.
-
-lemma union_comm : forall(X:'a t, Y:'a t),
-union X Y = union Y X.
-
-lemma union_add_aux : forall(X:'a t, Y:'a t, x: 'a),
-add x (union X Y) == union (add x X) Y.
-
-lemma union_add : forall(X:'a t, Y:'a t, x: 'a),
-add x (union X Y) = union (add x X) Y.
-
-lemma subset_union1 : forall (X Y : 'a t),
- X <= union X Y.
-
- (* local *) pred P_subset_union (X : 'a t) = forall(Y : 'a t),
- X <= Y => exists (Z : 'a t), Y = union X Z.
-
-lemma subset_union2 : forall (X : 'a t, Y : 'a t),
- X <= Y => exists (Z : 'a t), Y = union X Z
+lemma union_comm: forall (X Y:'a set),
+  union X Y = union Y X
 proof.
- intros X.
- cut H0 : (P_subset_union X).
- apply Set_ind<:'a>(P_subset_union,_,_,X).
- trivial.
- intros S x H H0.
- cut H1 : (forall (Y : 'a t), (add x S)<= Y => (exists (Z : 'a t), Y = union (add x S) Z)).
- intros Y H1.
- cut H2 : (S <= Y).
- trivial.
- cut H3 : (forall(Y : 'a t),
- S <= Y => exists (Z : 'a t), Y = union S Z).
- trivial.
- cut H4 : (exists (Z : 'a t), Y = union S Z).
- apply H3(Y,_).
- assumption.
- elim H4.
- intros Z H5.
- trivial.
- trivial.
- trivial.
+intros X Y;
+  apply extentionality<:'a> ((union X Y),(union Y X),_);
+  trivial.
+save.
+
+lemma union_add: forall (x:'a) X Y,
+  add x (union X Y) = union (add x X) Y
+proof.
+intros x X Y;
+  apply extentionality<:'a> ((add x (union X Y)),(union (add x X) Y),_);
+  trivial.
+save.
+
+lemma subset_union1: forall (X Y:'a set),
+  X <= union X Y.
+
+pred (* local *) cP_subset_union(X:'a set) = forall Y,
+  X <= Y => exists Z, Y = union X Z.
+
+lemma subset_union2: forall (X Y:'a set),
+  X <= Y => exists Z, Y = union X Z
+proof.
+intros X;cut H0: (cP_subset_union X).
+  apply Set_ind<:'a>(cP_subset_union,_,_,X).
+    trivial.
+    intros x S H H0;cut H1: (forall Y, (add x S) <= Y => (exists Z, Y = union (add x S) Z)).
+      intros Y H1;cut H2 : (S <= Y).
+        trivial.
+        cut H3: (forall Y, S <= Y => exists Z, Y = union S Z).
+          trivial.
+          cut H4: (exists Z, Y = union S Z).
+            apply H3(Y,_);assumption.
+            elim H4;intros Z H5;trivial.
+      trivial.
+  trivial.
 save.
 
 
-  (* local *) pred P_union_card1( X : 'a t) = forall(Y :'a t),
+pred (* local *) cP_union_card1(X:'a set) = forall Y,
   card (union X Y) <= card(X) + card(Y).
-
-lemma union_card1 : forall (X:'a t, Y:'a t),
- card (union X Y) <= card (X) + card(Y)
+lemma union_card1: forall (X Y:'a set),
+  card (union X Y) <= card (X) + card(Y)
 proof.
- intros X.
- cut H : (P_union_card1 X).
- apply Set_ind<:'a>(P_union_card1,_,_,X);trivial.
- trivial.
+intros X;cut H: (cP_union_card1 X);
+[ apply Set_ind<:'a>(cP_union_card1,_,_,X);trivial |
+  trivial ].
 save.
 
-pred P_union_card2( Y : 'a t) = forall(X:'a t),
- card X <= card (union X Y).
-
-lemma union_card2 : forall (Y:'a t, X:'a t),
- card X <= card (union X Y)
+pred (* local *) cP_union_card2(Y:'a set) = forall (X:'a set),
+  card X <= card (union X Y).
+lemma union_card2: forall (Y X:'a set),
+  card X <= card (union X Y)
 proof. 
- intros Y.
- cut H : (P_union_card2 Y).
- apply Set_ind<:'a>(P_union_card2,_,_,Y). 
- trivial.
- intros S x H H1.
- cut H0 : (forall(X:'a t),
- card X <= card (union X (add x S))).
- intros X.
- cut H2: (card X <= card (union X S)).
- trivial.
- cut H3: (card (union X S) <= card (union X (add x S))).
- cut H4: (card (union X (add x S)) = card (add x (union X S))).
- trivial.
- trivial.
- trivial.
- trivial.
- trivial.
+intros Y;cut H: (cP_union_card2 Y).
+  apply Set_ind<:'a>(cP_union_card2,_,_,Y). 
+    trivial.
+    intros x S H H1;cut H0 : (forall X, card X <= card (union X (add x S))).
+      intros X;cut H2: (card X <= card (union X S)).
+        trivial.
+        cut H3: (card (union X S) <= card (union X (add x S))).
+          cut H4: (card (union X (add x S)) = card (add x (union X S)));trivial.
+          trivial.
+      trivial.
+    trivial.
 save.
 
-
-  (* subset card *)
-
-lemma susbset_card : forall (Y : 'a t, X : 'a t),
- X <= Y => (card X) <= (card Y)
+lemma subset_card: forall (X Y:'a set),
+  X <= Y => (card X) <= (card Y)
 proof.
- intros Y X H.
- cut H0: (exists (Z : 'a t), Y = union X Z).
- trivial.
- elim H0.
- intros Z H1.
- cut H2: (card X <= card (union X Z)).
- trivial.
- trivial.
+intros X Y H;cut H0: (exists Z, Y = union X Z).
+  trivial.
+  elim H0;intros Z H1;cut H2: (card X <= card (union X Z));
+    trivial.
 save.
 
-  (* intersection *)
-axiom inter_mem : forall(X:'a t, Y:'a t, x: 'a),
- mem x (inter X Y) <=> (mem x X && mem x Y).
+(* intersection *)
+axiom inter_mem: forall (x:'a) X Y,
+  mem x (inter X Y) <=> (mem x X /\ mem x Y).
 
-lemma inter_empty : forall(X :'a t),
-inter X empty = empty
+lemma inter_empty: forall (X:'a set),
+  inter X empty = empty
 proof.
- intros X.
- cut H : (inter X empty == empty).
- trivial.
- trivial.
+intros X;
+  apply extentionality<:'a> ((inter X empty),empty,_);
+  trivial.
 save.
 
-lemma inter_comm : forall(X:'a t, Y:'a t),
-inter X Y = inter Y X 
+lemma inter_comm: forall (X Y:'a set),
+  inter X Y = inter Y X
 proof.
- intros X Y.
- cut H: (inter X Y == inter Y X).
- trivial.
- trivial.
+intros X Y;
+  apply extentionality<:'a> ((inter X Y),(inter Y X),_);
+  trivial.
 save.
 
-lemma inter_add : forall(X:'a t, Y:'a t, x: 'a),
-add x (inter X Y) = inter (add x X) (add x Y)
+lemma inter_add: forall (x:'a) X Y,
+  add x (inter X Y) = inter (add x X) (add x Y)
 proof.
- intros X Y x;cut ext_eq: (add x (inter X Y) == inter (add x X) (add x Y)).
-   cut H: (forall y, mem y (add x (inter X Y)) = mem y (inter (add x X) (add x Y)));trivial.
- trivial.
+intros x X Y;
+  apply extentionality<:'a> ((add x (inter X Y)),(inter (add x X) (add x Y)),_);
+  cut ext: (forall y, mem y (add x (inter X Y)) = mem y (inter (add x X) (add x Y)));trivial.
 save.
 
-lemma inter_add2 :forall(X : 'a t, Y : 'a t, x : 'a),
-mem x Y =>
-add x (inter X Y) = inter (add x X)  Y
+lemma inter_add2: forall (x:'a) X Y,
+  mem x Y => add x (inter X Y) = inter (add x X)  Y
 proof.
- intros X Y x H.
- cut H0: (add x (inter X Y) == inter (add x X)  Y).
- trivial.
- trivial.
+intros x X Y x_in_Y;
+  apply extentionality<:'a> ((add x (inter X Y)),(inter (add x X)  Y),_);
+  trivial.
 save.
 
 
-lemma inter_add3 :forall(X : 'a t, Y : 'a t, x : 'a),
- !mem x Y =>
-(inter X Y) = inter (add x X)  Y
+lemma inter_add3: forall (x:'a) X Y,
+  !mem x Y => (inter X Y) = inter (add x X) Y
 proof.
- intros X Y x H.
- cut H0: ((inter X Y) == inter (add x X)  Y).
- trivial.
- trivial.
+intros x X Y x_nin_Y;
+  apply extentionality<:'a> ((inter X Y),(inter (add x X) Y),_);
+  trivial.
 save.
 
-lemma subset_inter : forall (X Y : 'a t),
- inter X Y <= X.
+lemma subset_inter: forall (X Y:'a set),
+  inter X Y <= X.
 
-lemma card_inter : forall (X Y : 'a t),
- card (inter X Y) <= card X.
+lemma card_inter: forall (X Y:'a set),
+  card (inter X Y) <= card X.
 
-pred P_union_inter(X: 'a t) = forall(Y : 'a t),
- card(union X Y) + card(inter X Y) = card(X) + card(Y).
+pred (*local *) cP_union_inter(X:'a set) = forall Y,
+  card (union X Y) + card (inter X Y) = card X + card Y.
 
-lemma card_union_inter : forall (X Y: 'a t),
- card(union X Y) + card(inter X Y) = card(X) + card(Y)
+lemma card_union_inter: forall (X Y:'a set),
+  card (union X Y) + card (inter X Y) = card X + card Y
 proof. 
- intros X.
- cut H: (P_union_inter X).
- apply Set_ind<:'a>(P_union_inter,_,_, X).
- trivial.
- intros S x H H0.
- cut H1 : (forall (Y : 'a t),
- card(union (add x S) Y) + card(inter (add  x S) Y) = card(add x S) + card(Y)).
- intros Y.
- cut H8: (card(union S Y) + card(inter S Y) = card(S) + card(Y)).
- trivial.
- cut H2 : (mem x Y =>
- card(union (add x S) Y) + card(inter (add  x S) Y) = card(add x S) + card(Y)).
- intros H3.
- cut H4: (card (add x (inter S Y)) = card(inter (add x S) Y)).
- cut H5: (add x (inter S Y) = (inter (add x S) Y)).
- trivial.
- trivial.
- cut H5: (!mem x (inter S Y)).
- trivial.
- cut H6 : (card(inter (add  x S) Y) = 1 + card (inter S Y)).
- trivial.
- cut H7: (card(add x S) = 1 + card S).
- trivial.
- trivial.
- cut H3 : (!mem x Y =>
- card(union (add x S) Y) + card(inter (add  x S) Y) = card(add x S) + card(Y)).
- intros H4.
- cut H5: (card (inter S Y) = card(inter (add x S) Y)).
- trivial.
- cut H6: (!mem x (union S Y)).
- trivial.
- cut H7: (card(union(add x S) Y) = 1 + card(union S Y)).
- trivial.
- trivial.
- trivial.
- trivial.
- trivial.
+intros X;cut IH: (cP_union_inter X).
+  apply Set_ind<:'a>(cP_union_inter,_,_, X).
+    trivial.
+    intros x S H H0;cut H1: (forall Y, card (union (add x S) Y) + card (inter (add x S) Y) =
+                                         card (add x S) + card Y).
+      intros Y;cut H8: (card (union S Y) + card (inter S Y) = card S + card Y).
+        trivial.
+        cut H2: (mem x Y => card(union (add x S) Y) + card (inter (add x S) Y) = card (add x S) + card Y).
+          intros H3;cut H4: (card (add x (inter S Y)) = card (inter (add x S) Y)).
+            cut H5: (add x (inter S Y) = (inter (add x S) Y));trivial.
+            cut H5: (!mem x (inter S Y)).
+              trivial.
+              cut H6: (card (inter (add x S) Y) = 1 + card (inter S Y)).
+                trivial.
+                cut H7: (card (add x S) = 1 + card S);trivial.
+          cut H3: (!mem x Y => card (union (add x S) Y) + card (inter (add x S) Y) =
+                                 card (add x S) + card Y).
+            intros H4;cut H5: (card (inter S Y) = card (inter (add x S) Y)).
+              trivial.
+              cut H6: (!mem x (union S Y)).
+                trivial.
+                cut H7: (card (union (add x S) Y) = 1 + card (union S Y));trivial.
+      trivial.
+    trivial.
+  trivial.
 save.
 
 require import Real.
@@ -390,12 +325,12 @@ require import Distr.
 
 (* Uniform distribution on a (finite) set *)
 theory Duni.
-  op duni: 'a t -> 'a distr.
+  op duni: 'a set -> 'a distr.
 
   axiom supp_def: forall (x:'a) X, in_supp x (duni X) <=> mem x X.
 
-  axiom mu_def: forall (X:'a t) P, 
-    !is_empty X => 
+  axiom mu_def: forall (X:'a set) P, 
+    !is_empty X =>
        mu (duni X) P = (card (filter P X))%r / (card X)%r. 
 
   axiom mu_def_empty: forall (P:'a cPred), 
@@ -407,13 +342,13 @@ theory Duni.
   axiom mu_x_def_nin: forall (x:'a) X, 
     !mem x X => mu_x (duni X) x = 0%r.
 
-  axiom mu_weight: forall (X:'a t), 
+  axiom mu_weight: forall (X:'a set), 
      !is_empty X => mu_weight (duni X) = 1%r.
 end Duni.
 
 (* Restriction of a distribution (sub-distribution) *)
 theory Drestr.
-  op drestr: ('a distr,'a t) -> 'a distr.
+  op drestr: ('a distr,'a set) -> 'a distr.
  
   axiom supp_def: forall (x:'a) d X, 
      in_supp x (drestr d X) <=> in_supp x d /\ !mem x X.
@@ -427,12 +362,12 @@ theory Drestr.
     mu_x (drestr d X) x = 0%r.
 
   axiom mu_weight: forall (d:'a distr) X, 
-    mu_weight (drestr d X) = mu_weight d - mu d (Pmem X).
+    mu_weight (drestr d X) = mu_weight d - mu d (cPmem X).
 end Drestr.
 
 (* Scaled Restriction of a Distribution *)
 theory Dexcepted.
-  op [\] (d:'a distr, X:'a t): 'a distr =
+  op [\] (d:'a distr,X:'a set): 'a distr =
     Dscale.dscale (Drestr.drestr d X). 
 
   lemma supp_def: forall (x:'a) d X,
@@ -445,8 +380,8 @@ theory Dexcepted.
   save.
     
   lemma mu_x_def: forall (x:'a) d X,
-     mu_x (d \ X) x = (in_supp x (d \ X)) ? mu_x d x / (mu_weight d - mu d (Pmem X)) : 0%r.
+     mu_x (d \ X) x = (in_supp x (d \ X)) ? mu_x d x / (mu_weight d - mu d (cPmem X)) : 0%r.
 
-  lemma mu_weight_def: forall (d:'a distr, X:'a t),
-    mu_weight (d \ X) = (mu_weight d = mu d (Pmem X)) ? 0%r : 1%r.
+  lemma mu_weight_def: forall (d:'a distr) X,
+    mu_weight (d \ X) = (mu_weight d = mu d (cPmem X)) ? 0%r : 1%r.
 end Dexcepted.
